NewFMap.map: generalized definition, simplified proofs.

theories/newth/NewFMap.ec
@@ -446,55 +446,43 @@ proof.
 qed.
 
 (* -------------------------------------------------------------------- *)
-op map (f : 'a -> 'b -> 'b) (m : ('a, 'b) fmap) =
+op map (f : 'a -> 'b -> 'c) (m : ('a, 'b) fmap) =
   oflist (map (fun (x : 'a * 'b) => (x.`1,f x.`1 x.`2)) (elems m))
   axiomatized by mapE.
 
-(* TODO: Move me *)
-lemma map_fst_map (s : ('a * 'b) list) (f : 'a -> 'b -> 'b):
-    map fst (map (fun (x : 'a * 'b) => (x.`1,f x.`1 x.`2)) s)
-  = map fst s.
-proof. by elim s. qed.
+lemma dom_map (m : ('a,'b) fmap) (f : 'a -> 'b -> 'c) x:
+  mem (dom (map f m)) x <=> mem (dom m) x.
+proof.
+  rewrite mapE dom_oflist domE mem_oflist.
+  by elim (elems m)=> //= [[a b] l] /= ->.
+qed.
 
-lemma perm_eq_elems_map (m : ('a, 'b) fmap) (f : 'a -> 'b -> 'b):
+lemma perm_eq_elems_map (m : ('a, 'b) fmap) (f : 'a -> 'b -> 'c):
   perm_eq (map (fun (x : 'a * 'b) => (x.`1,f x.`1 x.`2)) (elems m))
           (elems (map f m)).
 proof.
   pose F := fun (x : 'a * 'b) => (x.`1,f x.`1 x.`2).
   apply @(perm_eq_trans (reduce (map F (elems m)))).
     rewrite -{1}@(reduce_reduced (map F (elems m))) 2:perm_eq_refl //.
-    by rewrite /F map_fst_map; apply/uniq_keys.
+    have ->: forall s, map fst (map F s) = map fst s by elim.
+    exact/uniq_keys.
   by rewrite mapE; apply/oflistK.
 qed.
 
-lemma mem_elems_map (m : ('a, 'b) fmap) (f : 'a -> 'b -> 'b) x y:
+lemma mem_elems_map (m : ('a, 'b) fmap) (f : 'a -> 'b -> 'c) x y:
       mem (map (fun (x : 'a * 'b) => (x.`1,f x.`1 x.`2)) (elems m)) (x,y)
   <=> mem (elems (map f m)) (x,y).
 proof. by apply/perm_eq_mem/perm_eq_elems_map. qed.
 
-lemma mem_map_map_elems (f : 'a -> 'b -> 'b) (f' : ('a * 'b) -> 'c) (m : ('a, 'b) fmap) a:
-      mem (map f' (map (fun (x : 'a * 'b) => (x.`1,f x.`1 x.`2)) (elems m))) a
-  <=> mem (map f' (elems (map f m))) a.
-proof. by apply/perm_eq_mem/perm_eq_map/perm_eq_elems_map. qed.
-
-lemma assoc_elems_map (m : ('a, 'b) fmap) (f: 'a -> 'b -> 'b) x:
-    assoc (map (fun (x : 'a * 'b) => (x.`1,f x.`1 x.`2)) (elems m)) x
-  = assoc (elems (map f m)) x.
-proof. by apply/perm_eq_assoc/perm_eq_elems_map/uniq_keys. qed.
-
-lemma dom_map (f : 'a -> 'b -> 'b) (m : ('a, 'b) fmap) x:
-  mem (dom (map f m)) x <=> mem (dom m) x.
-proof. by rewrite !mem_domE -mem_map_map_elems map_fst_map. qed.
-
-lemma mapP (f : 'a -> 'b -> 'b) (m : ('a, 'b) fmap) x:
+lemma mapP (f : 'a -> 'b -> 'c) (m : ('a, 'b) fmap) x:
   (map f m).[x] = omap (f x) m.[x].
 proof.
   pose F := fun (x : 'a * 'b) => (x.`1,f x.`1 x.`2).
   case (mem (dom (map f m)) x)=> h //=.
     case {-1}((map f m).[x]) (eq_refl (map f m).[x])=> [nh | y].
       by move: h; rewrite in_dom nh.
-    rewrite getE -mem_assoc_uniq 1:uniq_keys // -mem_elems_map mapP=> [[a b]] /=.
-    by rewrite mem_assoc_uniq 1:uniq_keys // -getE andC=> [[<<- ->>]] ->.
+    rewrite getE -mem_assoc_uniq 1:uniq_keys// -mem_elems_map mapP=> [[a b]] /=.
+    by rewrite mem_assoc_uniq 1:uniq_keys// -getE andC=> [[<<- ->>]] ->.
   have:= h; rewrite dom_map=> h'.
   by move: h h'; rewrite !in_dom /= => -> ->.
 qed.
